code/ecdsap256/Hacl.Impl.P256.Core.fst
@@ -512,6 +512,194 @@ let montgomery_ladder #a p q scalar tempBuffer =
       Lib.LoopCombinators.unfold_repeati 256 (spec_ml h0) (acc h0) (uint_v i)
     )
 
+(* prime = 2**256 - 2**224 + 2**192 + 2**96 -1
+
+def norm(p):    
+    x, y, z = p
+    z2i = power_mod(z * z, -1, prime)
+    z3i = power_mod(z * z * z, -1, prime)
+    return ((x * z2i) % prime, (y * z3i) % prime, 1)
+
+def toD(x):
+    return x * power_mod (2 ** 256, 1, prime) % prime
+
+def fromD(x):
+    return x * power_mod (2 ** 256, prime - 2, prime) % prime
+
+def toFakeAffine(p):
+    x, y = p 
+    multiplier = power_mod (2 ** 256, prime - 2, prime) 
+    x = x * multiplier * multiplier % prime
+    y = y * multiplier * multiplier * multiplier % prime
+    return (x, y)
+
+p256 = 0xFFFFFFFF00000001000000000000000000000000FFFFFFFFFFFFFFFFFFFFFFFF
+a256 = p256 - 3
+b256 = 0x5AC635D8AA3A93E7B3EBBD55769886BC651D06B0CC53B0F63BCE3C3E27D2604B
+gx = 0x6B17D1F2E12C4247F8BCE6E563A440F277037D812DEB33A0F4A13945D898C296
+gy = 0x4FE342E2FE1A7F9B8EE7EB4A7C0F9E162BCE33576B315ECECBB6406837BF51F5
+qq = 0xFFFFFFFF00000000FFFFFFFFFFFFFFFFBCE6FAADA7179E84F3B9CAC2FC632551
+FF = GF(p256)
+
+EC = EllipticCurve([FF(a256), FF(b256)])
+
+EC.set_order(qq)
+
+G = EC(FF(gx), FF(gy))
+
+def printf(p):
+    x, y = p 
+    for i in range(4):
+        print("u64 " + str(hex((Integer(x) >> (i * 64)) % 2 ** 64)) + "; ")
+    for i in range(4):
+        print("u64 " + str (hex((Integer(y) >> (i * 64)) % 2 ** 64)) + "; ")
+    
+
+for i in range(16):
+    pxD = i * G.xy()[0]
+    pyD = i * G.xy()[1]
+    printf (toFakeAffine((pxD, pyD)))
+
+ *)
+
+inline_for_extraction noextract
+let points_radix_16_list : x:list uint64{List.Tot.length x == 128} =
+  let open FStar.Mul in 
+  [@inline_let]
+  let x = [ 
+    u64 0x0; u64 0x0; u64 0x0; u64 0x0; 
+    u64 0x0; u64 0x0; u64 0x0; u64 0x0; 
+
+u64 0x1fb38ab1388ad777; 
+u64 0x1dfee06615fa309d; 
+u64 0xfcac986c3afea4a7; 
+u64 0xdf65c2da29fb821a; 
+u64 0xeff44e23f63f8f6d; 
+u64 0xaa02cd3ed4b681a4; 
+u64 0xdd5fda3363818af8; 
+u64 0xfc53bc2629fbf0b3; 
+u64 0x12631d721b91beea; 
+u64 0x5f73f2d3a11a09f8; 
+u64 0xac41f54484d5fcd8; 
+u64 0x86578e5c56025df4; 
+u64 0x577c956b15ed6b5a; 
+u64 0xb59c5f77982d848; 
+u64 0xb7c5e2c190fcdcc2; 
+u64 0x7d64d13ef1c91ffd; 
+u64 0xd40c2d6273f9d9f1; 
+u64 0x4dc6f628063ef17c; 
+u64 0x498e81df7ab17aa5; 
+u64 0xabb2a5026f17173c; 
+u64 0x4a3d7527f6739ef3; 
+u64 0xd941003268184c91; 
+u64 0xd2d458b8d401508b; 
+u64 0xb7437ab810ac5451; 
+u64 0x5256d9bdab491252; 
+u64 0x972d326eb1084c12; 
+u64 0xc3e96455e2ec3bfa; 
+u64 0xb75c723b549a10ff; 
+u64 0x9d9185f9f8a18961; 
+u64 0x2200a07b8589ba82; 
+u64 0x637b9d96fd4e9f5e; 
+u64 0xce75bfb2575e6cfa; 
+u64 0x7dd4477db8b77c7d; 
+u64 0x80818a776e5503b0; 
+u64 0x6fc7d58fb59581d; 
+u64 0xd899fb87efe43022; 
+u64 0x23b9912111694135; 
+u64 0x7e5de7bac33fa1c8; 
+u64 0xb3b83722a70e7d43; 
+u64 0xf06cfecbfb9bb38f; 
+u64 0xaa39277dfa93656; 
+u64 0x3dabb6cce67c5201; 
+u64 0x473ffb8bf1f94677; 
+u64 0xb9f0b93637453e56; 
+u64 0x8fce12ec20958fb2; 
+u64 0xcc16d74ff7786061; 
+u64 0x3678438a8235d096; 
+u64 0xe39ea044f06b43f6; 
+u64 0xbb40bdb5775c9950; 
+u64 0xd244a74cdc703cdd; 
+u64 0x83dc1b8a6105dd53; 
+u64 0x38d9d50d49ef0437; 
+u64 0x58be44eba6096472; 
+u64 0x960afaec386fa5c5; 
+u64 0x1440032e000134b9; 
+u64 0x601e721454d6ba96; 
+u64 0x79ec42228671b9b6; 
+u64 0xfdc00dc48df9e25c; 
+u64 0x44500833d71d2e77; 
+u64 0x2bda4c3c0bc103d5; 
+u64 0x51528408aa925d53; 
+u64 0xefcb55b9c2f3a37d; 
+u64 0x9f28f6bb9846c915; 
+u64 0xe1547ce1d8340e55; 
+u64 0x97e310c1995b3ed2; 
+u64 0xed861937196256e6; 
+u64 0x1c6762abff2c65f2; 
+u64 0x268345e0978fcedd; 
+u64 0x35ca2e572b784881; 
+u64 0x28ac888da0acd1b7; 
+u64 0x305640dc06a41baf; 
+u64 0x997c6fd2cb671bfb; 
+u64 0xf40d9eaf4a31e15a; 
+u64 0x8991dd7d54cfe03a; 
+u64 0x4889a3463a8deb0c; 
+u64 0x4cbf48092cd0a1fa; 
+u64 0xc6965c4fbe18fb8c; 
+u64 0x1d499d0cb216fa84; 
+u64 0x8d5fe52c705dd3eb; 
+u64 0x812b268f84313b34; 
+u64 0x313b58808261591a; 
+u64 0xc2c322508f53d933; 
+u64 0xa49ef3f95094ed1b; 
+u64 0x13e326786e98c63; 
+u64 0x34be8167cd460429; 
+u64 0x698a328099a6b31; 
+u64 0xb9be3ba51b0c922d; 
+u64 0xe59cca03f7674ed; 
+u64 0x4fbf7e505d3aca7c; 
+u64 0x2f4f8ba62020715; 
+u64 0x840502262ac1ec42; 
+u64 0xb8e0532775197de7; 
+u64 0x9142a358cf4e9b4b; 
+u64 0xc86a3c567e5d8626; 
+u64 0xd4051282b4a7992a; 
+u64 0xe7573c5999e3974e; 
+u64 0xd814a606da7bd76b; 
+u64 0x15604730f38cb788; 
+u64 0xbd195f868fbdd6c4; 
+u64 0xdb96f5b00a51d3f7; 
+u64 0xe1385c8a9b507fea; 
+u64 0x878e27813ee7310; 
+u64 0x6d7d8b12aea7e096; 
+u64 0x54978ad11e2f5cca; 
+u64 0x49fffd6c3c4d07d4; 
+u64 0x703638f71fab7a5d; 
+u64 0xbed6e367fcc73960; 
+u64 0x215e161835a61d75; 
+u64 0xe52288a5e87a660b; 
+u64 0xf1d127ee3c802cb5; 
+u64 0xccde3c6aafc46044; 
+u64 0xdc11c08ef14cff32; 
+u64 0x29216f9ceca46668; 
+u64 0x22e584a3b2891c5e; 
+u64 0xe6deecd7810f6d87; 
+u64 0x6aff4b94a55659a3; 
+u64 0x12b59bb6d2e9f876; 
+u64 0x27ed01943aa02eab; 
+u64 0x8d6d420841f57075; 
+u64 0xe7b47285ef60a461;  
+  ] in
+  x
+
+
+
+
+inline_for_extraction
+let points_radix_16 : x: glbuffer uint64 128ul {witnessed #uint64 #(size 128) x (Lib.Sequence.of_list points_radix_16_list) /\ recallable x} =
+    createL_global points_radix_16_list
+
 
 
 let getScalar #a scalar i = 
@@ -525,8 +713,8 @@ let getScalar #a scalar i =
   let open Hacl.Impl.P256.Q.PrimitivesMasking in 
   let bitShift = logand i (u32 1) in 
 
-  let mask = to_u32 (cmovznz01 0xf0 0x0f bitShift) in  
-  let shiftMask = to_u32 (cmovznz01 0x4 0x0 bitShift) in
+  let mask = to_u32 (cmovznz01  0xf0 0x0f  bitShift) in  
+  let shiftMask = to_u32 (cmovznz01  0x4 0x0 bitShift) in
 
   let result = logand word mask in 
   let result = shift_right result shiftMask in 
@@ -536,11 +724,10 @@ let getScalar #a scalar i =
   
 
 
-let montgomery_ladder_step_radix #buf_type p tempBuffer t scalar i = 
-  let i = 63ul -. i in 
-  let bits: uint32 = getScalar scalar i in 
+let montgomery_ladder_step_radix p tempBuffer scalar i =  
+  let bits: uint32 = getScalar scalar (i) in 
 
-  let pointToAdd = sub t (bits *. size 12) (size 8) in 
+  let pointToAdd = sub points_radix_16 (bits *. size 8) (size 8) in 
   
   point_double p p tempBuffer;
   point_double p p tempBuffer;
@@ -552,6 +739,31 @@ let montgomery_ladder_step_radix #buf_type p tempBuffer t scalar i =
 
 
 
+
+inline_for_extraction noextract
+val montgomery_ladder_2: #buf_type: buftype -> p: point -> 
+  scalar: lbuffer_t buf_type uint8 (size 32) -> 
+  tempBuffer:  lbuffer uint64 (size 88)  -> 
+  Stack unit
+  (requires fun h -> True )
+  (ensures fun h0 _ h1 -> modifies (loc p |+| loc tempBuffer) h0 h1)
+
+let montgomery_ladder_2 #a p scalar tempBuffer =  
+ let h0 = ST.get() in 
+
+  [@inline_let]
+  let spec_ml h0 = _ml_step (as_seq h0 scalar) in 
+
+  [@inline_let] 
+  let acc (h:mem) : GTot (point_nat_prime) = (fromDomainPoint(point_prime_to_coordinates (as_seq h p)))  in 
+
+  [@inline_let]
+  let inv h (i: nat {i <= 64}) = True in 
+
+  for 0ul 64ul inv 
+    (fun i -> let h2 = ST.get() in
+      montgomery_ladder_step_radix p tempBuffer scalar i
+    )
 
 
 
@@ -651,6 +863,8 @@ val scalarMultiplication_t: #t:buftype -> p: point -> result: point ->
 
 
 let scalarMultiplication_t #t p result scalar tempBuffer  = 
+(* 
+
     let h0 = ST.get() in 
   let q = sub tempBuffer (size 0) (size 12) in 
   zero_buffer q;
@@ -662,7 +876,23 @@ let scalarMultiplication_t #t p result scalar tempBuffer  =
     lemma_point_to_domain h0 h2 p result;
     lemma_pif_to_domain h2 q;
   norm q result buff; 
+    lemma_coord h3 q *)
+
+    let h0 = ST.get() in 
+  let q = sub tempBuffer (size 0) (size 12) in 
+  zero_buffer q;
+  let buff = sub tempBuffer (size 12) (size 88) in 
+  pointToDomain p result;
+    let h2 = ST.get() in 
+  montgomery_ladder_2 result scalar buff;
+    let h3 = ST.get() in 
+    lemma_point_to_domain h0 h2 p result;
+    lemma_pif_to_domain h2 q;
+  norm q result buff; 
     lemma_coord h3 q
+
+
+
 
 let scalarMultiplicationL = scalarMultiplication_t #MUT
 
@@ -723,7 +953,7 @@ let uploadBasePoint p =
   assert_norm (1 + pow2 64 * 18446744069414584320 + pow2 64 * pow2 64 * 18446744073709551615 + pow2 64 * pow2 64 * pow2 64 * 4294967294 = 26959946660873538059280334323183841250350249843923952699046031785985) 
 
 
-
+(*
 let scalarMultiplicationWithoutNorm p result scalar tempBuffer = 
   let h0 = ST.get() in 
   let q = sub tempBuffer (size 0) (size 12) in 
@@ -762,6 +992,52 @@ let secretToPublicWithoutNorm result scalar tempBuffer =
       let h1 = ST.get() in 
       lemma_pif_to_domain h1 q; 
     montgomery_ladder q basePoint scalar buff; 
+    copy_point q result;
+  pop_frame()  
+
+*)
+
+
+
+
+let scalarMultiplicationWithoutNorm p result scalar tempBuffer = 
+  let h0 = ST.get() in 
+  let q = sub tempBuffer (size 0) (size 12) in 
+  zero_buffer q;
+  let buff = sub tempBuffer (size 12) (size 88) in 
+  pointToDomain p result;
+    let h2 = ST.get() in 
+  montgomery_ladder_2 result scalar buff;
+  copy_point q result;  
+    let h3 = ST.get() in 
+    lemma_point_to_domain h0 h2 p result;
+    lemma_pif_to_domain h2 q
+    
+
+let secretToPublic result scalar tempBuffer = 
+  push_frame(); 
+       let basePoint = create (size 12) (u64 0) in 
+    (* uploadBasePoint basePoint; *)
+      let q = sub tempBuffer (size 0) (size 12) in 
+      let buff = sub tempBuffer (size 12) (size 88) in 
+    zero_buffer q; 
+      let h1 = ST.get() in 
+      lemma_pif_to_domain h1 q;
+    montgomery_ladder_2 q scalar buff; 
+    norm q result buff;  
+  pop_frame()
+
+
+let secretToPublicWithoutNorm result scalar tempBuffer = 
+    push_frame(); 
+      let basePoint = create (size 12) (u64 0) in 
+    uploadBasePoint basePoint;
+      let q = sub tempBuffer (size 0) (size 12) in 
+      let buff = sub tempBuffer (size 12) (size 88) in 
+    zero_buffer q; 
+      let h1 = ST.get() in 
+      lemma_pif_to_domain h1 q; 
+    montgomery_ladder_2 basePoint scalar buff; 
     copy_point q result;
   pop_frame()  
 
