code/ecdsap256/Hacl.Impl.P256.Core.fsti
@@ -145,10 +145,9 @@ val getScalar: #buf_type: buftype -> scalar: lbuffer_t buf_type uint8 (size 32) 
     (ensures fun h0 _ h1 -> True)
 
 
-val montgomery_ladder_step_radix:  #buf_type: buftype ->
+val montgomery_ladder_step_radix: 
   p: point -> tempBuffer: lbuffer uint64 (size 88) -> 
-  t: lbuffer uint64 (size 8 *! size 16) ->
-  scalar: lbuffer_t buf_type uint8 (size 32) -> 
+  scalar:  lbuffer uint8 (size 32)-> 
   i:size_t{v i < 256} -> 
   Stack unit
   (requires fun h -> live h p /\live h tempBuffer /\ live h scalar /\
