code/ecdsap256/Hacl.Impl.P256.MixedPointAdd.fsti
@@ -11,8 +11,12 @@ open Spec.P256.Definitions
 open Spec.P256.MontgomeryMultiplication
 open Spec.P256
 
+
+#set-options "--z3rlimit 150" 
+
 inline_for_extraction
-type pointAffine = lbuffer uint64 (size 8)
+type pointAffine = glbuffer uint64 (size 8)
+
 
 val point_add_mixed: p: point -> q: pointAffine -> result: point -> tempBuffer: lbuffer uint64 (size 88) -> 
    Stack unit (requires fun h -> live h p /\ live h q /\ live h result /\ live h tempBuffer /\ 
@@ -22,8 +26,8 @@ val point_add_mixed: p: point -> q: pointAffine -> result: point -> tempBuffer: 
     as_nat h (gsub p (size 8) (size 4)) < prime /\ 
     as_nat h (gsub p (size 0) (size 4)) < prime /\ 
     as_nat h (gsub p (size 4) (size 4)) < prime /\
-    as_nat h (gsub q (size 0) (size 4)) < prime /\ 
-    as_nat h (gsub q (size 4) (size 4)) < prime
+    as_nat_il h (gsub q (size 0) (size 4)) < prime /\ 
+    as_nat_il h (gsub q (size 4) (size 4)) < prime
 ) 
    (ensures fun h0 _ h1 -> 
      modifies (loc tempBuffer |+| loc result) h0 h1 /\ 
@@ -32,14 +36,13 @@ val point_add_mixed: p: point -> q: pointAffine -> result: point -> tempBuffer: 
      as_nat h1 (gsub result (size 4) (size 4)) < prime /\
      (
        let pX, pY, pZ = gsub p (size 0) (size 4), gsub p (size 4) (size 4), gsub p (size 8) (size 4) in 
-       let qX, qY = gsub q (size 0) (size 4), gsub q (size 4) (size 4) in 
+       let qX, qY = Lib.Buffer.gsub q (size 0) (size 4), Lib.Buffer.gsub q (size 4) (size 4) in 
        let x3, y3, z3 = gsub result (size 0) (size 4), gsub result (size 4) (size 4), gsub result (size 8) (size 4) in 
-       
        let pxD, pyD, pzD = fromDomain_ (as_nat h0 pX), fromDomain_ (as_nat h0 pY), fromDomain_ (as_nat h0 pZ) in 
-       let qxD, qyD = fromDomain_ (as_nat h0 qX), fromDomain_ (as_nat h0 qY) in 
+       let qxD, qyD = fromDomain_ (as_nat_il h0 qX), fromDomain_ (as_nat_il h0 qY) in 
        let x3D, y3D, z3D = fromDomain_ (as_nat h1 x3), fromDomain_ (as_nat h1 y3), fromDomain_ (as_nat h1 z3) in
       
        let xN, yN, zN = point_add_mixed (pxD, pyD, pzD) (qxD, qyD) in 
-       x3D == xN /\ y3D == yN /\ z3D == zN)
+       x3D == xN /\ y3D == yN /\ z3D == zN) 
    )
 
